coupling_inv : restructure template algorithm from CSSOp to CSS_insertOp

coupling_inv.v
@@ -64,27 +64,31 @@ Section Coupling_Template.
 
   Definition traverse : val :=
     rec: "tr" "p" "n" "k" :=
-      match: (findNext "n" "k") with
-        NONE => ("p", "n")
+      match: Fst (findNext "n" "k") with
+        NONE => (("p", "n"), Snd (findNext "n" "k"))
       | SOME "n'" =>
         lockNode "n'";; unlockNode "p";; "tr" "n" "n'" "k"
       end.
 
-  Definition CSSOp (Ψ: dOp) (root: Node) : val :=
+  Definition CSS_insertOp (root: Node) : val :=
     λ: "k",
     lockNode #root;;
-    let: "n0" := (findNext #root "k") in
+    let: "n0" := Fst (findNext #root "k") in
     match: "n0" with
       NONE => ""
     | SOME "n0" =>
       lockNode "n0";;
-      let: "pn" := traverse #root "n0" "k" in
-      let: "p" := Fst "pn" in
-      let: "n" := Snd "pn" in
-      let: "m" := alloc #() in
-      let: "res" := (decisiveOp Ψ) "p" "n" "k" in
-      unlockNode "p";; unlockNode "n";; "res" end.
-
+      let: "tr_res" := traverse #root "n0" "k" in
+      let: "b" := Snd "tr_res" in
+      if: "b" then 
+        #false
+      else
+        let: "pn" := Fst "tr_res" in 
+        let: "p" := Fst "pn" in
+        let: "n" := Snd "pn" in
+        let: "m" := alloc #() in
+        let: "res" := (decisiveOp insertOp) "p" "n" "k" in
+        unlockNode "p";; unlockNode "n";; "res" end.
 
   (** Assumptions on the implementation made by the template proofs.
    * Matching definitions can be found in GRASShopper file list-coupling.spl *)
@@ -93,19 +97,19 @@ Section Coupling_Template.
   Parameter node : Node → Node → inset_flowint_ur K → gset K → iProp.
 
   (* The following assumption is justified by the fact that GRASShopper uses a
-   * first-order separation logic. *)
+   * root-order separation logic. *)
   Parameter node_timeless_proof : ∀ root n I C, Timeless (node root n I C).
   Instance node_timeless root n I C: Timeless (node root n I C).
   Proof. apply node_timeless_proof. Qed.
 
   (* Spatial part of node predicate. *)
-  Parameter hrep_spatial : Node → iProp.
+  Parameter hrepSpatial : Node → iProp.
 
   (* The node-local invariant. 
    * See list-coupling.spl for the corresponding GRASShopper definition.*)
   (* TODO there's a slight discrepancy between this and grasshopper. *)
   Definition nodeinv root n (In : inset_flowint_ur K) Cn : Prop :=
-    n ∈ domm In
+    domm In = {[n]}
     ∧ Cn ⊆ keyset K In n
     ∧ (∀ k : K, default 0 (inf In n !! k) ≤ 1)
     ∧ (n = root → ∀ k1 : K, k1 ∈ KS → in_outsets K k1 In).
@@ -137,15 +141,13 @@ Section Coupling_Template.
     pose proof (intComp_valid_proj2 _ _ VI) as V23.
     pose proof (intComp_unfold_inf_1 _ _ VI n) as inf_I1.
     pose proof (intComp_unfold_inf_1 _ _ V23) as inf_I2.
-    destruct NI as (n_in_I2 & _ & inf_bound & _).
+    destruct NI as (domm_I2 & _ & inf_bound & _).
     assert (n ∈ domm I2 ∪ domm I3) as n_in_I23 by set_solver.
     pose proof (intComp_unfold_inf_2 _ _ VI n) as inf_I23.
     rewrite intComp_dom in inf_I23.
     apply inf_I23 in n_in_I23 as n_inf_I23.
     unfold cmra_op, flowintRA, cmra_car, K_multiset at 5, K_multiset at 5 in n_inf_I23.
-    pose proof (I_inf_out root) as (root_out & _).
-    assert (root = root) by reflexivity.
-    pose proof (root_out H0 k) as root_out_k.
+    pose proof (I_inf_out k k_in_KS) as root_out_k.
 
     assert (default 0 (inf I n !! k) ≠ 0).
     rewrite e.
@@ -162,7 +164,7 @@ Section Coupling_Template.
     rewrite root_out_k.
     simpl in H0.
     simpl.
-    naive_solver. done.
+    naive_solver.
     pose proof (lookup_op _ _ (inf I n) (out I1 n) k) as inf_I23_def.
 
     rewrite IDef in inf_I23_def.
@@ -173,7 +175,8 @@ Section Coupling_Template.
     rewrite <- n_inf_I23 in inf_I23_def.
     unfold cmra_op, flowintRA, cmra_car in IDef.
     rewrite <- IDef in inf_I23_def.
-
+    
+    assert (n ∈ domm I2) as n_in_I2 by set_solver.
     pose proof (inf_I2 n n_in_I2) as n_inf_I2.
     pose proof (lookup_op _ _ (inf (I2 ⋅ I3) n) (out I3 n) k) as inf_I2_def.
     unfold cmra_op, flowintRA, cmra_car, nzmap_total_lookup in inf_I2_def.
@@ -208,7 +211,7 @@ Section Coupling_Template.
     rewrite <- Heqx1 in inf_I2_def.
     lia.
     all: trivial.
-  Qed.  
+  Qed.
 
 
   (** Helper functions specs *)
@@ -220,23 +223,36 @@ Section Coupling_Template.
   Parameter findNext_spec : ∀ (n: Node) (k: K) (In : inset_flowint_ur K) (C: gset K) root,
      ⊢ ({{{ node root n In C ∗ ⌜in_inset K k In n⌝ }}}                
            findNext #n #k
-       {{{ (succ: bool) (np: Node),
-              RET (match succ with true => (SOMEV #np) | false => NONEV end);
-               node root n In C ∗ (match succ with true => ⌜in_outset K k In np⌝ |
-                                          false => ⌜¬in_outsets K k In⌝ ∗ ⌜n ≠ root⌝ end) }}})%I.
+       {{{ (succ: bool) (np: Node) (res: bool),
+              RET (match succ with true => ((SOMEV #np), #res) | false => (NONEV, #res) end);
+                  node root n In C ∗ ⌜res ↔ k ∈ C⌝ 
+               ∗ (match succ with true  => ⌜in_outset K k In np⌝
+                                | false => ⌜¬in_outsets K k In⌝ ∗ ⌜n ≠ root⌝ end) }}})%I.
 
-  Parameter decisiveOp_insert_spec : ∀ dop root (p n m: Node) (k: K) (Ip In: inset_flowint_ur K) (Cp Cn: gset K),
-     ⊢ ({{{ node root p Ip Cp ∗ node root n In Cn ∗ hrep_spatial m ∗ ⌜n ≠ root⌝ ∗ ⌜m ≠ root⌝
-                          ∗ ⌜in_inset K k Ip p⌝ ∗ ⌜in_outset K k Ip n ⌝ ∗ ⌜¬in_outsets K k In⌝ }}}
-           decisiveOp dop #p #n #k
+  Parameter decisiveOp_insert_spec : ∀ root (p n m: Node) (k: K) (Ip In: inset_flowint_ur K) (Cp Cn: gset K),
+     ⊢ ({{{       ⌜k ∈ KS⌝ 
+                ∗ ⌜keyset K Ip p ## keyset K In n⌝ 
+                ∗ node root p Ip Cp 
+                ∗ node root n In Cn
+                ∗ hrepSpatial m
+                ∗ ⌜✓ (Ip ⋅ In)⌝ 
+                ∗ ⌜out (Ip ⋅ In) m = 0%CCM⌝  
+                ∗ ⌜m ≠ root⌝ 
+                ∗ ⌜n ≠ root⌝ 
+                ∗ ⌜k ∉ Cn⌝
+                ∗ ⌜in_outset K k Ip n⌝ 
+                ∗ ⌜in_inset K k Ip p⌝  
+                ∗ ⌜¬in_outsets K k In⌝ }}}
+                
+           decisiveOp insertOp #p #n #k
+           
        {{{ (Cp1 Cn1 Cm1: gset K) (Ip1 In1 Im1: flowintUR K_multiset) (res: bool), RET  #res;
                   node root p Ip1 Cp1
                 ∗ node root n In1 Cn1
                 ∗ node root m Im1 Cm1
-                ∗ Ψ dop k (Cp ∪ Cn) (Cp1 ∪ Cn1 ∪ Cm1) res
+                ∗ Ψ insertOp k (Cp ∪ Cn) (Cp1 ∪ Cn1 ∪ Cm1) res
                 ∗ ⌜contextualLeq _ (Ip ⋅ In) (Ip1 ⋅ In1 ⋅ Im1)⌝
                 ∗ ⌜inf (Ip1 ⋅ In1 ⋅ Im1) m = 0%CCM⌝
-                ∗ ⌜domm Ip1 = {[p]}⌝ ∗ ⌜domm In1 = {[n]}⌝ ∗ ⌜domm Im1 = {[m]}⌝
                 ∗ ⌜keyset K Ip1 p ## keyset K In1 n⌝
                 ∗ ⌜keyset K Ip1 p ## keyset K Im1 m⌝
                 ∗ ⌜keyset K Im1 m ## keyset K In1 n⌝
@@ -245,7 +261,7 @@ Section Coupling_Template.
   Parameter alloc_spec :
      ⊢ ({{{ True }}}
            alloc #()
-       {{{ (m: Node) (l:loc), RET #m; hrep_spatial m ∗ ⌜lockLoc m = l⌝ ∗ l ↦ #false }}})%I.
+       {{{ (m: Node) (l:loc), RET #m; hrepSpatial m ∗ ⌜lockLoc m = l⌝ ∗ l ↦ #false }}})%I.
 
 
   (** The concurrent search structure invariant *)
@@ -325,13 +341,13 @@ Section Coupling_Template.
         ∗ own γ_k (◯ prod (keyset K I_n n, C_n))
     }}}
       traverse #p #n #k @ ⊤
-    {{{ (p' n': Node) (Ns': gsetUR Node) (I_p' I_n': inset_flowint_ur K) (C_p' C_n': gset K),
-        RET (#p', #n');
+    {{{ (p' n': Node) (Ns': gsetUR Node) (I_p' I_n': inset_flowint_ur K) (C_p' C_n': gset K) (res: bool),
+        RET ((#p', #n'), #res);
         own γ_fp (◯ Ns') ∗ ⌜p' ∈ Ns'⌝ ∗ ⌜n' ∈ Ns'⌝ ∗ own γ (◯ I_p') ∗ ⌜domm I_p' = {[p']}⌝ ∗ own γ (◯ I_n')
         ∗ ⌜domm I_n' = {[n']}⌝ ∗ node root p' I_p' C_p' ∗ node root n' I_n' C_n' ∗ ⌜n' ≠ root⌝
         ∗ own γ_k (◯ prod (keyset K I_p' p', C_p'))
         ∗ own γ_k (◯ prod (keyset K I_n' n', C_n'))
-        ∗ ⌜in_inset K k I_p' p'⌝ ∗ ⌜in_outset K k I_p' n'⌝ ∗ ⌜¬in_outsets K k I_n'⌝
+        ∗ ⌜in_inset K k I_p' p'⌝ ∗ ⌜in_outset K k I_p' n'⌝ ∗ ⌜¬in_outsets K k I_n'⌝ ∗ ⌜res ↔ k ∈ C_n'⌝
     }}}.
   Proof.
     iIntros "(% & #HInv)". iIntros (Φ) "!# H HCont". iLöb as "IH" forall (Ns p n I_p I_n C_p C_n).
@@ -345,7 +361,7 @@ Section Coupling_Template.
       apply (flowint_inset_step I_p I_n k n); try done. set_solver. }
     iDestruct "H" as "(HIp & HIn)".
     wp_apply ((findNext_spec n k I_n C_n root) with "[Hnoden]"). iFrame "∗ % #".
-    iIntros (b n') "(Hnoden & Hb)". destruct b.
+    iIntros (b n' res) "(Hnoden & % & Hb)". rename H12 into Hres. destruct b.
     - iDestruct "Hb" as "%". wp_pures.
       wp_bind (lockNode _)%E.
       awp_apply (lockNode_spec n') without "HCont".
@@ -414,15 +430,18 @@ Section Coupling_Template.
       iExists I_p, C_p. iFrame "∗ # %". iIntros "Hc". wp_pures.
       iSpecialize ("IH" $! (domm I1) n n' I_n I_n' C_n C_n').
       iApply ("IH" with "[-Hc]"). iFrame "∗ # %". iNext. done.
-    - wp_pures. iDestruct "Hb" as "(% & %)". iSpecialize ("HCont" $! p n Ns I_p I_n C_p C_n).
-      iApply "HCont". iFrame "∗ # %".
+    - wp_pures. wp_bind (findNext _ _)%E.
+      wp_apply (findNext_spec with "[Hnoden]"). iFrame "∗ %".
+      iIntros (suc n0 res0)"(Hnoden & Hres & Hsuc)". iDestruct "Hb" as "(% & %)".
+      iDestruct "Hres" as "%". iSpecialize ("HCont" $! p n Ns I_p I_n C_p C_n).
+      destruct suc; wp_pures; iApply "HCont"; iFrame "∗ # %".    
   Qed.
 
-  Theorem searchStrOp_spec (γ γ_fp γ_k γ_c: gname) root (k: K) (dop: dOp):
+  Theorem searchStrOp_spec (γ γ_fp γ_k γ_c: gname) root (k: K):
     ⊢ ⌜k ∈ KS⌝ ∗ css γ γ_fp γ_k γ_c root -∗
     <<< ∀ (C: gset K), css_cont γ_c C >>>
-      CSSOp dop root #k @ ⊤ ∖ ↑N
-    <<< ∃ C' (res: bool), css_cont γ_c C' ∗ (Ψ dop k C C' res : iProp), RET #res >>>.
+      CSS_insertOp root #k @ ⊤ ∖ ↑N
+    <<< ∃ C' (res: bool), css_cont γ_c C' ∗ (Ψ insertOp k C C' res : iProp), RET #res >>>.
   Proof.
     iIntros "(% & #HInv)". iIntros (Φ) "AU". wp_lam. wp_bind (lockNode _)%E.
     awp_apply (lockNode_spec root). iInv "HInv" as ">H".
@@ -446,10 +465,13 @@ Section Coupling_Template.
     iExists I0, C0. iFrame "∗ # %".
     iApply "Hstar". iExists true. iFrame "∗ # %".
     wp_pures. wp_bind(findNext _ _)%E.
-    assert (in_inset K k If root). { unfold globalinv in H1. destruct H1 as [? [? [? ?]]].
-    specialize (H7 root). destruct H7 as [H7 _]. apply (inset_monotone I0 If Io k root); try done; set_solver. }
+    assert (in_inset K k If root). 
+    { unfold globalinv in H1. destruct H1 as [? [? [? ?]]].
+    specialize (H7 k). apply (inset_monotone I0 If Io k root); try done.
+    by apply H7. set_solver. }
     wp_apply ((findNext_spec root k If Cf root) with "[Hnodef]").
-    { iFrame "∗ # %". } iIntros (b n) "(Hnodef & Hb)".
+    { iFrame "∗ # %". } iIntros (b n res0) "(Hnodef & Hres & Hb)".
+    iDestruct "Hres" as %Hres.
     destruct b; last first. wp_pures. iDestruct "Hb" as "(% & %)".
     exfalso. apply H6. done. iDestruct "Hb" as "%". wp_pures.
     wp_bind (lockNode _)%E. awp_apply (lockNode_spec n). iInv "HInv" as ">H".
@@ -491,245 +513,291 @@ Section Coupling_Template.
     wp_apply ((traverse_spec γ γ_fp γ_k γ_c root k root n (domm I2) If Cf In Cn)
                  with "[] [HIf HCf Hnodef HIn HCn Hnoden]").
     iFrame "∗ # %". iFrame "∗ # %".
-    iIntros (p' n' Ns Ip' In' Cp' Cn') "(#HNs & % & % & HIp' & % & HIn' & % & Hnodep' & Hnoden'
+    iIntros (p' n' Ns Ip' In' Cp' Cn' res1) "(#HNs & % & % & HIp' & % & HIn' & % & Hnodep' & Hnoden'
                         & % & Hksp' & Hksn' & % & % & %)".
-    wp_pures. wp_apply (alloc_spec); first done.
-    iIntros (m lm) "(Hrepm & % & Hlm)". wp_pures. wp_bind (decisiveOp _ _ _ _)%E.
-    iApply fupd_wp. iInv "HInv" as ">H".
-    iDestruct "H" as (I3 C3) "(HKS & HInt & % & HFP & Hcont & Hstar)".
-    destruct (decide (m ∈ domm I3)). { rewrite (big_sepS_elem_of_acc _ (domm I3) m); last by eauto.
-    iDestruct "Hstar" as "(Hm & Hstar)". iDestruct "Hm" as (b) "(Hlockm & Hb)".
-    iEval (rewrite H25) in "Hlockm". iDestruct (mapsto_valid_2 with "Hlm Hlockm") as "%".
-    exfalso. done. }
-    assert (root ∈ domm I3). { apply globalinv_root_fp. done. }
-    assert (m ≠ root). { set_solver. }
-    iModIntro. iSplitL "HKS HInt HFP Hcont Hstar". iNext.
-    iExists I3, C3. iFrame "∗ # %". iModIntro.
-    wp_apply ((decisiveOp_insert_spec dop root p' n' m k Ip' In' Cp' Cn')
-          with "[Hnodep' Hnoden' Hrepm]"). { iFrame "∗ % #". }
-    iIntros (Cp'' Cn'' Cm'' Ip'' In'' Im'' res) "(Hnodep' & Hnoden' & Hnodem' & #HΨ & % & Hminf & H)".
-    iDestruct "H" as "(% & % & % & % & % & % & %)".
-    iDestruct "Hminf" as %Hminf. 
-    iApply fupd_wp. iInv "HInv" as ">H".
-    iDestruct "H" as (I4 C4) "(HKS & HInt & % & HFP & Hcont & Hstar)".
-    iMod "AU" as (C') "[Hc [_ Hclose]]". iEval (rewrite /css_cont) in "Hc".
-    iDestruct (auth_agree with "Hcont Hc") as %<-.
-
-    (* ------ keyset update -------*)
-    
-    iAssert (⌜Cp'' ⊆ keyset K Ip'' p'⌝)%I with "[Hnodep']" as "%".
-    { iPoseProof (node_implies_nodeinv with "[Hnodep']") as "H". iFrame.
-      iPureIntro. unfold contextualLeq in H29. destruct H29 as [_ [H29 _]].
-      by repeat apply cmra_valid_op_l in H29. iDestruct "H" as "(_ & %)".
-      unfold nodeinv in H38. destruct H38 as [_ [H38 ]]. by iPureIntro. } 
-    iAssert (⌜Cn'' ⊆ keyset K In'' n'⌝)%I with "[Hnoden']" as "%".
-    { iPoseProof (node_implies_nodeinv with "[Hnoden']") as "H". iFrame.
-      iPureIntro. unfold contextualLeq in H29. destruct H29 as [_ [H29 _]].
-      apply cmra_valid_op_l in H29. by apply cmra_valid_op_r in H29.
-      iDestruct "H" as "(_ & %)". unfold nodeinv in H39.
-      destruct H39 as [_ [H39 ]]. by iPureIntro. } 
-    iAssert (⌜Cm'' ⊆ keyset K Im'' m⌝)%I with "[Hnodem']" as "%".
-    { iPoseProof (node_implies_nodeinv with "[Hnodem']") as "H". iFrame.
-      iPureIntro. unfold contextualLeq in H29. destruct H29 as [_ [H29 _]].
+    wp_pures. destruct res1.
+    {  
+      iInv "HInv" as ">H".
+      iDestruct "H" as (I3 C3) "(HKS & HInt & % & HFP & Hcont & Hstar)".
+      iPoseProof (own_valid with "HKS") as "%".
+      iPoseProof (own_valid with "Hksn'") as "%".
+      iPoseProof ((auth_own_incl γ_k (prod (KS, C3)) _) with "[HKS Hksn']") as "%".
+      iFrame. rewrite auth_auth_valid in H26 *; intros H26.
+      rewrite auth_frag_valid in H27 *; intros H27.
+      pose proof (auth_ks_included (keyset K In' n') KS Cn' C3 H27 H26 H28).
+      iMod "AU" as (C') "[Hc [_ Hclose]]". iEval (rewrite /css_cont) in "Hc".
+      iDestruct (auth_agree with "Hcont Hc") as %<-.
+      wp_pures. 
+      iSpecialize ("Hclose" $! C3 false).
+      iMod ("Hclose" with "[Hc]") as "HΦ". iFrame.
+      unfold Ψ. iPureIntro. destruct H24 as (_ & H24).
+      assert (k ∈ Cn'). apply H24. done.
+      assert (Cn' ⊆ C3). destruct H29.
+      clear -H29. set_solver. destruct H29 as [a [b [_ [H29 _]]]].
+      clear -H29. set_solver. clear -H30 H31. split; set_solver.
+      iModIntro. iModIntro. iSplitR "HΦ". iNext. iExists I3, C3. iFrame "∗ %".
+      done.
+    }
+    {
+      wp_pures.      
+      wp_apply (alloc_spec); first done.
+      iIntros (m lm) "(Hrepm & % & Hlm)". wp_pures. wp_bind (decisiveOp _ _ _ _)%E.
+      iApply fupd_wp. iInv "HInv" as ">H".
+      iDestruct "H" as (I3 C3) "(HKS & HInt & % & HFP & Hcont & Hstar)".
+      destruct (decide (m ∈ domm I3)). { rewrite (big_sepS_elem_of_acc _ (domm I3) m); last by eauto.
+      iDestruct "Hstar" as "(Hm & Hstar)". iDestruct "Hm" as (b) "(Hlockm & Hb)".
+      iEval (rewrite H25) in "Hlockm". iDestruct (mapsto_valid_2 with "Hlm Hlockm") as "%".
+      exfalso. done. }
+      assert (root ∈ domm I3). { apply globalinv_root_fp. done. }
+      assert (m ≠ root). { set_solver. }
+      iPoseProof ((own_op γ (◯ Ip') (◯ In')) with "[HIp' HIn']") as "HIpn'"; first by eauto with iFrame.
+      iPoseProof (own_valid with "HIpn'") as "%". rename H29 into Valid_Ipn'.
+      rewrite -auth_frag_op in Valid_Ipn'. rewrite auth_frag_valid in Valid_Ipn' *; intros Valid_Ipn'.
+      iPoseProof ((own_op γ_k _ _) with "[Hksp' Hksn']") as "Hkspn'"; first by eauto with iFrame.
+      iPoseProof (own_valid with "Hkspn'") as "%". rename H29 into Valid_kspn'.
+      rewrite -auth_frag_op in Valid_kspn'. rewrite auth_frag_valid in Valid_kspn' *; intros Valid_kspn'.
+      unfold op, cmra_op in Valid_kspn'. simpl in Valid_kspn'.
+      unfold ucmra_op in Valid_kspn'. simpl in Valid_kspn'. repeat case_decide; try done .
+      rename H29 into Subset_c_ks_n'. rename H30 into Subset_c_ks_p'.
+      rename H31 into Disj_ks_pn'. rename H32 into Disj_c_pn'. iEval (rewrite -auth_frag_op) in "HIpn'".
+      iPoseProof ((auth_own_incl _ I3) with "[$HInt $HIpn']") as (Iw)"%". rename H29 into Valid_I3.
+      assert (out (Ip'⋅In') m = 0%CCM) as Out_zero_pn'.
+      { 
+        apply (intComp_out_zero Iw (Ip'⋅In') m).
+        rewrite intComp_comm. destruct H26 as [H26 _].
+        by rewrite <-Valid_I3.
+        rewrite intComp_comm. by rewrite <-Valid_I3.
+        rewrite intComp_comm. rewrite <-Valid_I3.
+        unfold globalinv in H26. destruct H26 as (_ & _ & H26 & _).
+        apply nzmap_eq. intros k0. pose proof (H26 k0 m).
+        unfold outset, dom_ms in H29. 
+        rewrite (nzmap_elem_of_dom_total) in H29 *; intros H29.
+        apply dec_stable in H29. by rewrite nzmap_lookup_empty. 
+      }    
+      iModIntro. iSplitL "HKS HInt HFP Hcont Hstar". iNext.
+      iExists I3, C3. iFrame "∗ # %". iModIntro. destruct H24 as [H24 Hk_not0].
+      assert (k ∉ Cn') as Hk_not1. { unfold not. apply Hk_not0. }
+      wp_apply ((decisiveOp_insert_spec root p' n' m k Ip' In' Cp' Cn')
+            with "[Hnodep' Hnoden' Hrepm]"). { iFrame "∗ % #". iPureIntro. set_solver. }
+      iIntros (Cp'' Cn'' Cm'' Ip'' In'' Im'' res) "(Hnodep' & Hnoden' & Hnodem' & #HΨ & % & Hminf & H)".
+      iDestruct "H" as "(% & % & % & %)".
+      iDestruct "Hminf" as %Hminf. 
+      iApply fupd_wp. iInv "HInv" as ">H".
+      iDestruct "H" as (I4 C4) "(HKS & HInt & % & HFP & Hcont & Hstar)".
+      iMod "AU" as (C') "[Hc [_ Hclose]]". iEval (rewrite /css_cont) in "Hc".
+      iDestruct (auth_agree with "Hcont Hc") as %<-.
+  
+      (* ------ keyset update -------*)
+      
+      iAssert (⌜Cp'' ⊆ keyset K Ip'' p' ∧ domm Ip'' = {[p']}⌝)%I with "[Hnodep']" as "%".
+      { iPoseProof (node_implies_nodeinv with "[Hnodep']") as "H". iFrame.
+        iPureIntro. unfold contextualLeq in H29. destruct H29 as [_ [H29 _]].
+        by repeat apply cmra_valid_op_l in H29. iDestruct "H" as "(_ & %)".
+        unfold nodeinv in H35. destruct H35 as [Hdom [H35 ]]. by iPureIntro. } 
+      iAssert (⌜Cn'' ⊆ keyset K In'' n' ∧ domm In'' = {[n']}⌝)%I with "[Hnoden']" as "%".
+      { iPoseProof (node_implies_nodeinv with "[Hnoden']") as "H". iFrame.
+        iPureIntro. unfold contextualLeq in H29. destruct H29 as [_ [H29 _]].
+        apply cmra_valid_op_l in H29. by apply cmra_valid_op_r in H29.
+        iDestruct "H" as "(_ & %)". unfold nodeinv in H36.
+        destruct H36 as [Hdom [H36 ]]. by iPureIntro. } 
+      iAssert (⌜Cm'' ⊆ keyset K Im'' m ∧ domm Im'' = {[m]}⌝)%I with "[Hnodem']" as "%".
+      { iPoseProof (node_implies_nodeinv with "[Hnodem']") as "H". iFrame.
+        iPureIntro. unfold contextualLeq in H29. destruct H29 as [_ [H29 _]].
       by repeat apply cmra_valid_op_r in H29. iDestruct "H" as "(_ & %)".
-      unfold nodeinv in H40. destruct H40 as [_ [H40 ]]. by iPureIntro. }
-    assert (Cp'' ## Cn''). { clear -H38 H39 H33. set_solver. }
-    assert (Cn'' ## Cm''). { clear -H40 H39 H35. set_solver. }
-    assert (Cm'' ## Cp''). { clear -H38 H40 H34. set_solver. }
-    iPoseProof ((own_op γ_k (◯ prod (keyset K Ip' p', Cp')) (◯ prod (keyset K In' n', Cn'))
-                      with "[Hksp' Hksn']")) as "H"; first by eauto with iFrame.
-    iEval (rewrite -auth_frag_op) in "H".
-    iPoseProof (own_valid with "H") as "%".
-    rewrite auth_frag_valid in H44 *; intros Hvprod.
-    unfold op, cmra_op in Hvprod. simpl in Hvprod. unfold ucmra_op in Hvprod.
-    simpl in Hvprod. repeat case_decide;
-        [ simpl | try exfalso; eauto | try exfalso; eauto | try exfalso; eauto | try exfalso; eauto].
-    assert (prod (keyset K Ip'' p', Cp'') ⋅ prod (keyset K In'' n', Cn'') ⋅ prod (keyset K Im'' m, Cm'')
-                 = prod (keyset K Ip'' p' ∪ keyset K In'' n' ∪ keyset K Im'' m, Cp'' ∪ Cn'' ∪ Cm'')).
-    { unfold op, prodOp. repeat case_decide; try done. exfalso. apply H55. set_solver by eauto.
-      exfalso. apply H54. clear - H33 H34 H35. set_solver by eauto. exfalso. apply H52. set_solver by eauto. }
-    assert (◯ (prod (keyset K Ip'' p', Cp'') ⋅ prod (keyset K In'' n', Cn'') ⋅ prod (keyset K Im'' m, Cm''))
-                 = ◯ (prod (keyset K Ip'' p' ∪ keyset K In'' n' ∪ keyset K Im'' m, Cp'' ∪ Cn'' ∪ Cm''))).
-    { rewrite H48. reflexivity. }
-    assert ((prod (keyset K Ip' p', Cp') ⋅ prod (keyset K In' n', Cn'))
-                  = prod (keyset K Ip' p' ∪ keyset K In' n', Cp' ∪ Cn')).
-    { unfold op, prodOp. repeat case_decide; try done. }
-    iPoseProof ((own_op γ (◯ Ip') (◯ In')) with "[HIp' HIn']") as "H'"; first by eauto with iFrame.
-    iPoseProof (own_valid with "H'") as "%". rewrite -auth_frag_op in H51.
-    assert (✓ (Ip' ⋅ In')). { apply (auth_frag_valid (◯ (Ip' ⋅ In'))). done. }
-    assert (in_inset K k In' n'). {
-      apply (flowint_inset_step Ip' In' k n'); try done. rewrite H20. clear. set_solver. }
-    assert (k ∈ keyset K In' n'). { apply keyset_def; try done. }
-    iMod ((ghost_update_keyset γ_k dop k (Cp' ∪ Cn') (Cp'' ∪ Cn'' ∪ Cm'') res
-                 (keyset K Ip' p' ∪ keyset K In' n') C4) with "[HKS H]") as "Hgks".
-    iEval (rewrite H50) in "H". iFrame "∗ # %". iPureIntro.
-    split. rewrite <-H36. clear -H38 H39 H40. set_solver. clear -H54. set_solver.
-    iDestruct "Hgks" as (C4') "(#HΨ' & HKS & H)". iEval (rewrite <-H36) in "H".
-    iAssert (own γ_k (◯ (prod (keyset K Ip'' p', Cp'') ⋅ prod (keyset K In'' n', Cn'') ⋅ prod (keyset K Im'' m, Cm''))))
-          with "[H]" as "Hv". { iEval (rewrite H48). done. }
-    iDestruct "Hv" as "((Hksp' & Hksn') & Hksm')".
-    iMod (auth_excl_update γ_c (C4') with "Hcont Hc") as "[Hcont Hc]".
-    clear - H0 node_implies_nodeinv node_sep_star p' n' Ns Ip' In' Cp'
-            Cn' H17 H18 H19 H20 H21 H22 H23 H24 m lm H25 Cp'' Cn'' Cm'' Ip''
-            In'' Im'' res H29 H30 H31 H32 Hminf I4 C4 H37 H51 H52 H53 H54 C4'.
-
-    (* ------ interface update -------*)
-
-    destruct (decide (m ∈ domm I4)). { rewrite (big_sepS_elem_of_acc _ (domm I4) m); last by eauto.
-    iDestruct "Hstar" as "(Hm & Hstar)". iDestruct "Hm" as (b) "(Hlockm & Hb)".
-    iEval (rewrite H25) in "Hlockm". iDestruct (mapsto_valid_2 with "Hlm Hlockm") as "%".
-    exfalso. done. }
-    assert (◯ Ip' ⋅ ◯ In' = ◯ (Ip' ⋅ In')).
-    by rewrite auth_frag_op. iEval (rewrite H1) in "H'". iCombine "HInt" "H'" as "Hownint".
-    iPoseProof (own_valid with "Hownint") as "%".
-    apply auth_both_valid in H2. destruct H2. destruct H2 as [Iz H2].
-    iDestruct "Hownint" as "[HInt H']".
-    destruct H29 as (Hvldpn & Hvldpnm & Hsub & Hinf & Hout).
-    assert (domm (Ip'' ⋅ In'' ⋅ Im'') = domm Ip'' ∪ domm In'' ∪ domm Im''). 
-    repeat rewrite (flowint_comp_fp); try done. by apply cmra_valid_op_l in Hvldpnm.
-    rewrite H30 H31 H32 in H4.
-    assert (m ∉ domm Iz). { apply leibniz_equiv in H2. rewrite H2 in n.
-    rewrite (flowint_comp_fp) in n. set_solver. apply leibniz_equiv_iff in H2.
-    rewrite <-H2. done. }
-    unfold globalinv in H37. destruct H37 as (Hv & H4root & H4out & H4in).
-    assert (out Iz m = 0%CCM).
-    { 
-      apply (intComp_out_zero (Ip'⋅In') Iz m). by rewrite <-H2.
-      rewrite <-H2. done. rewrite <-H2. apply nzmap_eq.
-      intros km. pose proof (H4out km m).
-      unfold outset, dom_ms in H6. rewrite (nzmap_elem_of_dom_total) in H6 *; intros.
-      apply dec_stable in H6. rewrite H6.
-      by rewrite nzmap_lookup_empty.
-    }    
-    iMod (own_updateP (flowint_update_P K_multiset I4 (Ip' ⋅ In') (Ip'' ⋅ In'' ⋅ Im'')) γ
-                          (● I4 ⋅ ◯ (Ip' ⋅ In')) with "[HInt H']") as (Io'') "H0".
-    {
-      rewrite H2.
-      apply (flowint_update K_multiset (Iz) (Ip' ⋅ In') (Ip'' ⋅ In'' ⋅ Im'')).
-      repeat split; try done. apply leibniz_equiv in H2. assert (H4valid := H3).
-      rewrite H2 in H3. apply intComposable_valid in H3. unfold intComposable in H3.
-      destruct H3 as (_ & _ & Hdisj & _). rewrite flowint_comp_fp in Hdisj; last first.
-      rewrite H2 in H4valid; by apply cmra_valid_op_l in H4valid.
-      rewrite H4. rewrite H19 H20 in Hdisj. clear -Hdisj H5. set_solver.
-      intros nf. rewrite flowint_comp_fp; try done. 
-      repeat rewrite (flowint_comp_fp); last by apply cmra_valid_op_l in Hvldpnm.
-      rewrite H30 H31 H32 H19 H20. intros Hnf. assert (nf = m). set_solver. replace nf.
-      unfold out in H6. done. done.
-    }
-    { try repeat rewrite own_op; iFrame. }
-    iPoseProof ((flowint_update_result γ I4 (Ip' ⋅ In') (Ip'' ⋅ In'' ⋅ Im''))
-                      with "H0") as (I') "(% & % & HIIpnm)".
-    iEval (rewrite own_op) in "HIIpnm". iDestruct "HIIpnm" as "(HI' & HIpnm'')".
-    iPoseProof ((own_valid γ (● I')) with "HI'") as "%".
-    iPoseProof (own_valid with "HIpnm''") as "%".
-    assert (✓ (Ip'' ⋅ In'' ⋅ Im'')) as HIpnmcheck.
-    { apply (auth_frag_valid (◯ (Ip'' ⋅ In'' ⋅ Im''))). done. }
-    iEval (rewrite auth_frag_op) in "HIpnm''".
-    iDestruct "HIpnm''" as "(HIpn'' & HIm'')".
-    iPoseProof (own_valid with "HIpn''") as "%".
-    assert (✓ (Ip'' ⋅ In'')) as HIpncheck.
-    { apply (auth_frag_valid (◯ (Ip'' ⋅ In''))). done. }
-    iEval (rewrite auth_frag_op) in "HIpn''".
-    iDestruct "HIpn''" as "(HIp'' & HIn'')".
-    destruct (decide (m ∈ domm I4)). { rewrite (big_sepS_elem_of_acc _ (domm I4) m); last by eauto.
-    iDestruct "Hstar" as "(Hm & Hstar)". iDestruct "Hm" as (b) "(Hlockm & Hb)".
-    iEval (rewrite H25) in "Hlockm". iDestruct (mapsto_valid_2 with "Hlm Hlockm") as "%".
-    exfalso. done. }
-    iMod (own_update γ_fp (● domm I4) (● (domm I4 ∪ {[m]}) ⋅ ◯ (domm I4 ∪ {[m]})) with "[HFP]") as "H".
-    { apply (auth_update_alloc (domm I4) (domm I4 ∪ {[m]}) (domm I4 ∪ {[m]})).
-      apply gset_local_update. set_solver. }
-    done. iDestruct "H" as "(HFP & #Hfp4)".
-    assert (domm I' = domm I4 ∪ {[m]}).
-    {
-      destruct H8 as [I_o H8]. destruct H8.
-      assert (domm I' = {[p']} ∪ {[n']} ∪ {[m]} ∪ domm I_o).
+      unfold nodeinv in H37. destruct H37 as [Hdom [H37 ]]. by iPureIntro. }
+      destruct H35 as [Sub_p Dom_p]. destruct H36 as [Sub_n Dom_n].
+      destruct H37 as [Sub_m Dom_m].
+      assert (Cp'' ## Cn'') as Disj_pn. { clear -Sub_p Sub_n H30. set_solver. }
+      assert (Cn'' ## Cm'') as Disj_nm. { clear -Sub_m Sub_n H32. set_solver. }
+      assert (Cm'' ## Cp'') as Disj_pm. { clear -Sub_p Sub_m H31. set_solver. }
+      iEval (rewrite -auth_frag_op) in "Hkspn'".
+      assert (prod (keyset K Ip'' p', Cp'') ⋅ prod (keyset K In'' n', Cn'') ⋅ prod (keyset K Im'' m, Cm'')
+                   = prod (keyset K Ip'' p' ∪ keyset K In'' n' ∪ keyset K Im'' m, Cp'' ∪ Cn'' ∪ Cm'')).
+      { unfold op, prodOp. repeat case_decide; try done. exfalso. apply H42. set_solver by eauto.
+        exfalso. apply H41. clear - H30 H31 H32. set_solver by eauto. exfalso. apply H39. set_solver by eauto. }
+      assert (◯ (prod (keyset K Ip'' p', Cp'') ⋅ prod (keyset K In'' n', Cn'') ⋅ prod (keyset K Im'' m, Cm''))
+                   = ◯ (prod (keyset K Ip'' p' ∪ keyset K In'' n' ∪ keyset K Im'' m, Cp'' ∪ Cn'' ∪ Cm''))).
+      { rewrite H35. reflexivity. }
+      assert ((prod (keyset K Ip' p', Cp') ⋅ prod (keyset K In' n', Cn'))
+                    = prod (keyset K Ip' p' ∪ keyset K In' n', Cp' ∪ Cn')).
+      { unfold op, prodOp. repeat case_decide; try done. }
+      assert (in_inset K k In' n'). {
+        apply (flowint_inset_step Ip' In' k n'); try done. rewrite H20. clear. set_solver. }
+      assert (k ∈ keyset K In' n'). { apply keyset_def; try done. }
+      iMod ((ghost_update_keyset γ_k insertOp k (Cp' ∪ Cn') (Cp'' ∪ Cn'' ∪ Cm'') res
+                   (keyset K Ip' p' ∪ keyset K In' n') C4) with "[HKS Hkspn']") as "Hgks".
+      iEval (rewrite comm) in "Hkspn'".             
+      iEval (rewrite H37) in "Hkspn'". iFrame "∗ # %". iPureIntro.
+      split. rewrite <-H33. clear -Sub_p Sub_n Sub_m. set_solver. clear -H39. set_solver.
+      iDestruct "Hgks" as (C4') "(#HΨ' & HKS & H)". iEval (rewrite <-H33) in "H".
+      iAssert (own γ_k (◯ (prod (keyset K Ip'' p', Cp'') ⋅ prod (keyset K In'' n', Cn'') ⋅ prod (keyset K Im'' m, Cm''))))
+            with "[H]" as "Hv". { iEval (rewrite H35). done. }
+      iDestruct "Hv" as "((Hksp' & Hksn') & Hksm')".
+      iMod (auth_excl_update γ_c (C4') with "Hcont Hc") as "[Hcont Hc]".
+      clear H39 H37 H36 H35 Disj_pm Disj_nm Disj_pn Sub_m Sub_n Sub_p H30 H31 H32 H33
+            Hk_not1 Hk_not0 Valid_I3 Out_zero_pn' Iw Valid_kspn' Disj_c_pn' Disj_ks_pn'
+            Subset_c_ks_p' Subset_c_ks_n' H27 n0 H26 C3 I3 H15 H14 H16 Iu H13 H12 H11 
+            Cn In H10 H9 H7 Io' HI2 H8 Hcheck C2 H6 Hres res0 n H5 H4 Io H3 Cf If 
+            H2 H1 C0.
+            
+      (* ------ interface update -------*)
+  
+      destruct (decide (m ∈ domm I4)). { rewrite (big_sepS_elem_of_acc _ (domm I4) m); last by eauto.
+      iDestruct "Hstar" as "(Hm & Hstar)". iDestruct "Hm" as (b) "(Hlockm & Hb)".
+      iEval (rewrite H25) in "Hlockm". iDestruct (mapsto_valid_2 with "Hlm Hlockm") as "%".
+      exfalso. done. }
+      assert (◯ Ip' ⋅ ◯ In' = ◯ (Ip' ⋅ In')).
+      by rewrite auth_frag_op. iCombine "HInt" "HIpn'" as "Hownint".
+      iPoseProof (own_valid with "Hownint") as "%".
+      apply auth_both_valid in H2. destruct H2. destruct H2 as [Iz H2].
+      iDestruct "Hownint" as "[HInt H']".
+      destruct H29 as (Hvldpn & Hvldpnm & Hsub & Hinf & Hout).
+      assert (domm (Ip'' ⋅ In'' ⋅ Im'') = domm Ip'' ∪ domm In'' ∪ domm Im''). 
+      repeat rewrite (flowint_comp_fp); try done. by apply cmra_valid_op_l in Hvldpnm.
+      rewrite Dom_p Dom_n Dom_m in H4.
+      assert (m ∉ domm Iz). { apply leibniz_equiv in H2. rewrite H2 in n.
+      rewrite (flowint_comp_fp) in n. set_solver. apply leibniz_equiv_iff in H2.
+      rewrite <-H2. done. }
+      unfold globalinv in H34. destruct H34 as (Hv & H4root & H4out & H4in).
+      assert (out Iz m = 0%CCM).
+      { 
+        apply (intComp_out_zero (Ip'⋅In') Iz m). by rewrite <-H2.
+        rewrite <-H2. done. rewrite <-H2. apply nzmap_eq.
+        intros km. pose proof (H4out km m).
+        unfold outset, dom_ms in H6. rewrite (nzmap_elem_of_dom_total) in H6 *; intros.
+        apply dec_stable in H6. rewrite H6.
+        by rewrite nzmap_lookup_empty.
+      }    
+      iMod (own_updateP (flowint_update_P K_multiset I4 (Ip' ⋅ In') (Ip'' ⋅ In'' ⋅ Im'')) γ
+                            (● I4 ⋅ ◯ (Ip' ⋅ In')) with "[HInt H']") as (Io'') "H0".
       {
-        subst I'. repeat rewrite flowint_comp_fp; try congruence; try done.
-        by apply (auth_auth_valid).
+        rewrite H2.
+        apply (flowint_update K_multiset (Iz) (Ip' ⋅ In') (Ip'' ⋅ In'' ⋅ Im'')).
+        repeat split; try done. apply leibniz_equiv in H2. assert (H4valid := H3).
+        rewrite H2 in H3. apply intComposable_valid in H3. unfold intComposable in H3.
+        destruct H3 as (_ & _ & Hdisj & _). rewrite flowint_comp_fp in Hdisj; last first.
+        rewrite H2 in H4valid; by apply cmra_valid_op_l in H4valid.
+        rewrite H4. rewrite H19 H20 in Hdisj. clear -Hdisj H5. set_solver.
+        intros nf. rewrite flowint_comp_fp; try done. 
+        repeat rewrite (flowint_comp_fp); last by apply cmra_valid_op_l in Hvldpnm.
+        rewrite Dom_p Dom_n Dom_m H19 H20. intros Hnf. assert (nf = m). set_solver. replace nf.
+        unfold out in H6. done. done.
       }
-      assert (domm I4 = {[p']} ∪ {[n']} ∪ domm I_o).
+      { try repeat rewrite own_op; iFrame. }
+      iPoseProof ((flowint_update_result γ I4 (Ip' ⋅ In') (Ip'' ⋅ In'' ⋅ Im''))
+                        with "H0") as (I') "(% & % & HIIpnm)".
+      iEval (rewrite own_op) in "HIIpnm". iDestruct "HIIpnm" as "(HI' & HIpnm'')".
+      iPoseProof ((own_valid γ (● I')) with "HI'") as "%".
+      iPoseProof (own_valid with "HIpnm''") as "%".
+      assert (✓ (Ip'' ⋅ In'' ⋅ Im'')) as HIpnmcheck.
+      { apply (auth_frag_valid (◯ (Ip'' ⋅ In'' ⋅ Im''))). done. }
+      iEval (rewrite auth_frag_op) in "HIpnm''".
+      iDestruct "HIpnm''" as "(HIpn'' & HIm'')".
+      iPoseProof (own_valid with "HIpn''") as "%".
+      assert (✓ (Ip'' ⋅ In'')) as HIpncheck.
+      { apply (auth_frag_valid (◯ (Ip'' ⋅ In''))). done. }
+      iEval (rewrite auth_frag_op) in "HIpn''".
+      iDestruct "HIpn''" as "(HIp'' & HIn'')".
+      destruct (decide (m ∈ domm I4)). { rewrite (big_sepS_elem_of_acc _ (domm I4) m); last by eauto.
+      iDestruct "Hstar" as "(Hm & Hstar)". iDestruct "Hm" as (b) "(Hlockm & Hb)".
+      iEval (rewrite H25) in "Hlockm". iDestruct (mapsto_valid_2 with "Hlm Hlockm") as "%".
+      exfalso. done. }
+      iMod (own_update γ_fp (● domm I4) (● (domm I4 ∪ {[m]}) ⋅ ◯ (domm I4 ∪ {[m]})) with "[HFP]") as "H".
+      { apply (auth_update_alloc (domm I4) (domm I4 ∪ {[m]}) (domm I4 ∪ {[m]})).
+        apply gset_local_update. set_solver. }
+      done. iDestruct "H" as "(HFP & #Hfp4)".
+      assert (domm I' = domm I4 ∪ {[m]}).
       {
-        subst I4. repeat rewrite flowint_comp_fp; try congruence; try done.
-      }
-      rewrite H13 H14.
-      clear. set_solver.
-    }
-    
-    assert (globalinv K root I'). {
-      apply (contextualLeq_impl_globalinv I4 I').
-      all : trivial.
-      unfold globalinv. repeat split; try done. apply H4in. apply H4in.
-      intros.
-      assert (n1 = m). { clear - H12 n0 H13. set_solver. } subst n1.
-      unfold inset. unfold dom_ms. unfold inf. case_eq (inf_map I' !! m); last first.
-      - intros Hm. unfold ccmunit, ccm_unit. simpl. unfold nzmap_dom. simpl. set_solver.
-      - intros k0 Hk0. simpl. destruct H8 as [Iz' [H8 ?]]. 
-        rewrite H8 in H2. apply intComp_cancelable in H2; last by rewrite H8 in H3.
-        apply leibniz_equiv in H2. subst Iz'.
-        assert (inf (Ip'' ⋅ In'' ⋅ Im'' ⋅ Iz) m = (inf (Ip'' ⋅ In''⋅ Im'') m) - (out Iz m))%CCM.
-        { apply intComp_inf_1. apply leibniz_equiv_iff in H14. rewrite <-H14.
-          by apply auth_auth_valid.
-          assert (domm (Ip'' ⋅ In'' ⋅ Im'') = domm Ip'' ∪ domm In'' ∪ domm Im''). 
-          repeat rewrite (flowint_comp_fp); try done. rewrite H2.
-          rewrite H32. clear. set_solver.
+        destruct H8 as [I_o H8]. destruct H8.
+        assert (domm I' = {[p']} ∪ {[n']} ∪ {[m]} ∪ domm I_o).
+        {
+          subst I'. repeat rewrite flowint_comp_fp; try congruence; try done.
+          by apply (auth_auth_valid).
         }
-        rewrite Hminf in H2. rewrite <-H14 in H2.
-        rewrite H6 in H2. rewrite ccm_pinv_unit in H2. unfold inf in H2. rewrite Hk0 in H2.
-        simpl in H2. rewrite H2. unfold ccmunit, lift_unit, nzmap_unit. simpl.
-        unfold nzmap_dom. simpl. set_solver.
-    }
-    iEval (rewrite <-H12) in "HFP". assert (domm I'∖ {[m]} = domm I4). 
-    { clear -n0 H12. set_solver. }
-
-    (* ------ updates over -------*)
-
-    iMod ("Hclose" with "[Hc]") as "HΦ". iFrame "∗ % #".
-    iModIntro. iSplitL "Hstar Hlm Hnodem' HKS Hcont HI' HIm'' HFP Hksm'". iNext. iExists I', C4'.
-    iFrame "∗ # %". rewrite (big_sepS_delete _ (domm I') m); last set_solver. iEval (rewrite H14).
-    iFrame. iExists false. iEval (rewrite H25). iFrame. iExists Im'', Cm''. eauto with iFrame.
-    iModIntro. wp_pures. wp_bind (unlockNode _)%E.
-
-    (* ------ linearization over -------*)
-
-    awp_apply (unlockNode_spec p') without "HΦ". iInv "HInv" as ">H".
-    iDestruct "H" as (I6 C6) "(HKS & HInt & % & HFP & Hcont & Hstar)".
-    iAssert (⌜p' ∈ domm I6⌝)%I with "[HFP]" as "%".
-    { iPoseProof ((auth_own_incl γ_fp (domm I6) Ns) with "[$]") as "%".
-      apply gset_included in H16.
-      iPureIntro. clear -H16 H17. set_solver. }
-    rewrite (big_sepS_elem_of_acc _ (domm I6) p'); last by eauto.
-    iDestruct "Hstar" as "[Hb Hstar]". iDestruct "Hb" as (b) "[Hlock Hb]".
-    destruct b; last first. { iDestruct "Hb" as (In0 Cn0) "(_ & _ & Hrep' & _)".
-    iAssert (⌜False⌝)%I with "[Hnodep' Hrep']" as %Hf. { iApply (node_sep_star root p' Ip'' In0 _ _).
-    iFrame. } exfalso. done. }
-    iAaccIntro with "Hlock". 
-    { iIntros. iModIntro. iFrame "∗". iNext. iExists I6, C6.
-      iFrame "∗ # %". iApply "Hstar". iExists true. iFrame. }
-    iIntros. iModIntro.
-    iSplitR "Hnoden' Hksn' HIn''". iNext. iExists I6, C6.
-    iFrame "∗ # %". iApply "Hstar". iExists false. iFrame. iExists Ip'', Cp''. iFrame "∗ %".
-
-    iIntros "HΦ".
-    wp_pures. wp_bind (unlockNode _)%E.
-    awp_apply (unlockNode_spec n') without "HΦ".
-    iInv "HInv" as ">H". iDestruct "H" as (I7 C7) "(HKS & HInt & % & HFP & Hcont & Hstar)".
-    iAssert (⌜n' ∈ domm I7⌝)%I with "[HFP]" as "%".
-    { iPoseProof ((auth_own_incl γ_fp (domm I7) Ns) with "[$]") as "%".
-      apply gset_included in H27.
+        assert (domm I4 = {[p']} ∪ {[n']} ∪ domm I_o).
+        {
+          subst I4. repeat rewrite flowint_comp_fp; try congruence; try done.
+        }
+        rewrite H13 H14.
+        clear. set_solver.
+      }
+      
+      assert (globalinv K root I'). {
+        apply (contextualLeq_impl_globalinv I4 I').
+        all : trivial.
+        unfold globalinv. repeat split; try done.
+        intros.
+        assert (n1 = m). { clear - H12 n0 H13. set_solver. } subst n1.
+        unfold inset. unfold dom_ms. unfold inf. case_eq (inf_map I' !! m); last first.
+        - intros Hm. unfold ccmunit, ccm_unit. simpl. unfold nzmap_dom. simpl. set_solver.
+        - intros k0 Hk0. simpl. destruct H8 as [Iz' [H8 ?]]. 
+          rewrite H8 in H2. apply intComp_cancelable in H2; last by rewrite H8 in H3.
+          apply leibniz_equiv in H2. subst Iz'.
+          assert (inf (Ip'' ⋅ In'' ⋅ Im'' ⋅ Iz) m = (inf (Ip'' ⋅ In''⋅ Im'') m) - (out Iz m))%CCM.
+          { apply intComp_inf_1. apply leibniz_equiv_iff in H14. rewrite <-H14.
+            by apply auth_auth_valid.
+            assert (domm (Ip'' ⋅ In'' ⋅ Im'') = domm Ip'' ∪ domm In'' ∪ domm Im''). 
+            repeat rewrite (flowint_comp_fp); try done. rewrite H2.
+            rewrite Dom_m. clear. set_solver.
+          }
+          rewrite Hminf in H2. rewrite <-H14 in H2.
+          rewrite H6 in H2. rewrite ccm_pinv_unit in H2. unfold inf in H2. rewrite Hk0 in H2.
+          simpl in H2. rewrite H2. unfold ccmunit, lift_unit, nzmap_unit. simpl.
+          unfold nzmap_dom. simpl. set_solver.
+      }
+      iEval (rewrite <-H12) in "HFP". assert (domm I'∖ {[m]} = domm I4). 
+      { clear -n0 H12. set_solver. }
+  
+      (* ------ updates over -------*)
+  
+      iMod ("Hclose" with "[Hc]") as "HΦ". iFrame "∗ % #".
+      iModIntro. iSplitL "Hstar Hlm Hnodem' HKS Hcont HI' HIm'' HFP Hksm'". iNext. iExists I', C4'.
+      iFrame "∗ # %". rewrite (big_sepS_delete _ (domm I') m); last set_solver. iEval (rewrite H14).
+      iFrame. iExists false. iEval (rewrite H25). iFrame. iExists Im'', Cm''. eauto with iFrame.
+      iModIntro. wp_pures. wp_bind (unlockNode _)%E.
+  
+      (* ------ linearization over -------*)
+  
+      awp_apply (unlockNode_spec p') without "HΦ". iInv "HInv" as ">H".
+      iDestruct "H" as (I6 C6) "(HKS & HInt & % & HFP & Hcont & Hstar)".
+      iAssert (⌜p' ∈ domm I6⌝)%I with "[HFP]" as "%".
+      { iPoseProof ((auth_own_incl γ_fp (domm I6) Ns) with "[$]") as "%".
+        apply gset_included in H16.
+        iPureIntro. clear -H16 H17. set_solver. }
+      rewrite (big_sepS_elem_of_acc _ (domm I6) p'); last by eauto.
+      iDestruct "Hstar" as "[Hb Hstar]". iDestruct "Hb" as (b) "[Hlock Hb]".
+      destruct b; last first. { iDestruct "Hb" as (In0 Cn0) "(_ & _ & Hrep' & _)".
+      iAssert (⌜False⌝)%I with "[Hnodep' Hrep']" as %Hf. { iApply (node_sep_star root p' Ip'' In0 _ _).
+      iFrame. } exfalso. done. }
+      iAaccIntro with "Hlock". 
+      { iIntros. iModIntro. iFrame "∗". iNext. iExists I6, C6.
+        iFrame "∗ # %". iApply "Hstar". iExists true. iFrame. }
+      iIntros. iModIntro.
+      iSplitR "Hnoden' Hksn' HIn''". iNext. iExists I6, C6.
+      iFrame "∗ # %". iApply "Hstar". iExists false. iFrame. iExists Ip'', Cp''. iFrame "∗ %".
+  
+      iIntros "HΦ".
+      wp_pures. wp_bind (unlockNode _)%E.
+      awp_apply (unlockNode_spec n') without "HΦ".
+      iInv "HInv" as ">H". iDestruct "H" as (I7 C7) "(HKS & HInt & % & HFP & Hcont & Hstar)".
+      iAssert (⌜n' ∈ domm I7⌝)%I with "[HFP]" as "%".
+      { iPoseProof ((auth_own_incl γ_fp (domm I7) Ns) with "[$]") as "%".
+        apply gset_included in H27.
       iPureIntro. clear -H18 H27. set_solver. }
-    rewrite (big_sepS_elem_of_acc _ (domm I7) n'); last by eauto.
-    iDestruct "Hstar" as "[Hb Hstar]". iDestruct "Hb" as (b) "[Hlock Hb]".
-    destruct b; last first. { iDestruct "Hb" as (In0 Cn0) "(_ & _ & Hrep' & _)".
-    iAssert (⌜False⌝)%I with "[Hnoden' Hrep']" as %Hf. { iApply (node_sep_star root n' In'' In0 _ _).
-    iFrame. } exfalso. done. }
-    iAaccIntro with "Hlock".
-    { iIntros. iModIntro. iFrame "∗ # %". iNext. iExists I7, C7.
-      iFrame "∗ # %". iApply "Hstar". iExists true. iFrame. }
-    iIntros. iModIntro.
-    iSplitL. iNext. iExists I7, C7.
-    iFrame "∗ # %". iApply "Hstar". iExists false. iFrame. iExists In'', Cn''. iFrame "∗ %".
-
-    iIntros "HΦ". wp_pures. done.
-  Qed.
+      rewrite (big_sepS_elem_of_acc _ (domm I7) n'); last by eauto.
+      iDestruct "Hstar" as "[Hb Hstar]". iDestruct "Hb" as (b) "[Hlock Hb]".
+      destruct b; last first. { iDestruct "Hb" as (In0 Cn0) "(_ & _ & Hrep' & _)".
+      iAssert (⌜False⌝)%I with "[Hnoden' Hrep']" as %Hf. { iApply (node_sep_star root n' In'' In0 _ _).
+      iFrame. } exfalso. done. }
+      iAaccIntro with "Hlock".
+      { iIntros. iModIntro. iFrame "∗ # %". iNext. iExists I7, C7.
+        iFrame "∗ # %". iApply "Hstar". iExists true. iFrame. }
+      iIntros. iModIntro.
+      iSplitL. iNext. iExists I7, C7.
+      iFrame "∗ # %". iApply "Hstar". iExists false. iFrame. iExists In'', Cn''. iFrame "∗ %".
+  
+      iIntros "HΦ". wp_pures. done.
+      }
+    Qed.
 
 End Coupling_Template.
